RocqOfRust/revm/revm_interpreter/instructions/simulate/host/sstore.v
@@ -1,6 +1,7 @@
 Require Import simulate.RocqOfRust.
 Require Import alloy_primitives.links.aliases.
 Require Import core.links.array.
+Require Import core.links.result.
 Require Import revm.revm_context_interface.links.host.
 Require Import revm.revm_context_interface.links.journaled_state.
 Require Import revm.revm_context_interface.simulate.host.
@@ -9,10 +10,12 @@ Require Import revm.revm_interpreter.gas.simulate.constants.
 Require Import revm.revm_interpreter.instructions.links.host.sstore.
 Require Import revm.revm_interpreter.instructions.simulate.macros.
 Require Import revm.revm_interpreter.links.gas.
+Require Import revm.revm_interpreter.links.instruction_context.
 Require Import revm.revm_interpreter.links.interpreter.
 Require Import revm.revm_interpreter.links.instruction_result.
 Require Import revm.revm_interpreter.links.interpreter_types.
 Require Import revm.revm_interpreter.simulate.gas.
+Require Import revm.revm_interpreter.simulate.interpreter.
 Require Import revm.revm_interpreter.simulate.interpreter_types.
 Require Import revm.revm_primitives.links.hardfork.
 Require Import revm.revm_primitives.simulate.hardfork.
@@ -34,52 +37,54 @@ Definition sstore
   let target :=
     IInterpreterTypes.(InterpreterTypes.InputsTrait_for_Input).(InputTraits.target_address)
       interpreter.(Interpreter.input) in
-  let '(result, host) := IHost.(Host.sstore) host target index value in
-  match result with
-  | None =>
-    let control :=
-      IInterpreterTypes.(InterpreterTypes.LoopControl_for_Control).(LoopControl.set_instruction_result)
-        interpreter.(Interpreter.control)
-        instruction_result.InstructionResult.FatalExternalError in
-    (interpreter <| Interpreter.control := control |>, host)
-  | Some state_load =>
-
   let spec_id :=
     IInterpreterTypes.(InterpreterTypes.RuntimeFlag_for_RuntimeFlag).(RuntimeFlag.spec_id)
       interpreter.(Interpreter.runtime_flag) in
-  let gas :=
-    IInterpreterTypes.(InterpreterTypes.LoopControl_for_Control).(LoopControl.gas)
-      .(RefStub.projection) interpreter.(Interpreter.control) in
   if (Impl_SpecId.is_enabled_in spec_id SpecId.ISTANBUL)
-      && (i[gas.(Gas.remaining)] <=? i[constants.CALL_STIPEND]) then
-    let control :=
-      IInterpreterTypes.(InterpreterTypes.LoopControl_for_Control).(LoopControl.set_instruction_result)
-        interpreter.(Interpreter.control)
-        instruction_result.InstructionResult.ReentrancySentryOOG in
-    (interpreter <| Interpreter.control := control |>, host)
+      && (i[Impl_Gas.remaining interpreter.(Interpreter.gas)] <=? i[constants.CALL_STIPEND]) then
+    (halt interpreter instruction_result.InstructionResult.ReentrancySentryOOG, host)
   else
-  let spec_id :=
-    IInterpreterTypes.(InterpreterTypes.RuntimeFlag_for_RuntimeFlag).(RuntimeFlag.spec_id)
-      interpreter.(Interpreter.runtime_flag) in
-  let vals_ref : '& SStoreResult.t :=
-    Ref.immediate Pointer.Kind.Ref state_load.(StateLoad.data) in
   gas_macro interpreter
-    (calc.sstore_cost spec_id vals_ref state_load.(StateLoad.is_cold))
+    (calc.static_sstore_cost spec_id)
     (fun interpreter => (interpreter, host)) (fun interpreter =>
+  if Impl_SpecId.is_enabled_in spec_id SpecId.BERLIN then
+    let skip_cold :=
+      i[Impl_Gas.remaining interpreter.(Interpreter.gas)] <?
+      COLD_SLOAD_COST_ADDITIONAL.(Integer.value) in
+    let '(result, host) :=
+      IHost.(Host.sstore_skip_cold_load) host target index value skip_cold in
+    match result with
+    | Result.Ok state_load =>
+        let vals_ref : '& SStoreResult.t :=
+          Ref.immediate Pointer.Kind.Ref state_load.(StateLoad.data) in
+        gas_macro interpreter
+          (calc.dyn_sstore_cost spec_id vals_ref state_load.(StateLoad.is_cold))
+          (fun interpreter => (interpreter, host)) (fun interpreter =>
 
-  let spec_id :=
-    IInterpreterTypes.(InterpreterTypes.RuntimeFlag_for_RuntimeFlag).(RuntimeFlag.spec_id)
-      interpreter.(Interpreter.runtime_flag) in
-  let refund := calc.sstore_refund spec_id vals_ref in
-  let gas :=
-    IInterpreterTypes.(InterpreterTypes.LoopControl_for_Control).(LoopControl.gas)
-      .(RefStub.projection) interpreter.(Interpreter.control) in
-  let gas := Impl_Gas.record_refund gas refund in
-  let control :=
-    IInterpreterTypes.(InterpreterTypes.LoopControl_for_Control).(LoopControl.gas)
-      .(RefStub.injection) interpreter.(Interpreter.control) gas in
-  (interpreter <| Interpreter.control := control |>, host))
-  end)).
+        let refund := calc.sstore_refund spec_id vals_ref in
+        let gas := Impl_Gas.record_refund interpreter.(Interpreter.gas) refund in
+        (interpreter <| Interpreter.gas := gas |>, host))
+    | Result.Err LoadError.ColdLoadSkipped =>
+        (halt_oog interpreter, host)
+    | Result.Err LoadError.DBError =>
+        (halt_fatal interpreter, host)
+    end
+  else
+    let '(result, host) := IHost.(Host.sstore) host target index value in
+    match result with
+    | Some state_load =>
+        let vals_ref : '& SStoreResult.t :=
+          Ref.immediate Pointer.Kind.Ref state_load.(StateLoad.data) in
+        gas_macro interpreter
+          (calc.dyn_sstore_cost spec_id vals_ref state_load.(StateLoad.is_cold))
+          (fun interpreter => (interpreter, host)) (fun interpreter =>
+
+        let refund := calc.sstore_refund spec_id vals_ref in
+        let gas := Impl_Gas.record_refund interpreter.(Interpreter.gas) refund in
+        (interpreter <| Interpreter.gas := gas |>, host))
+    | None =>
+        (halt_fatal interpreter, host)
+    end))).
 
 Lemma sstore_eq
     {WIRE H : Set} `{Link WIRE} `{Link H}
@@ -96,10 +101,14 @@ Lemma sstore_eq
     (host : H) :
   let ref_interpreter := make_ref 0 in
   let ref_host := make_ref (A := H) 1 in
+  let context := {|
+    instruction_context.InstructionContext.interpreter := ref_interpreter;
+    instruction_context.InstructionContext.host := ref_host;
+  |} in
   let result := sstore interpreter host in
   {{
     SimulateM.eval_f
-      (run_sstore run_InterpreterTypes_for_WIRE run_Host_for_H ref_interpreter ref_host)
+      (run_sstore run_InterpreterTypes_for_WIRE run_Host_for_H context)
       [interpreter; host]%stack 🌲
     (
       Output.Success tt,
@@ -107,80 +116,4 @@ Lemma sstore_eq
     )
   }}.
 Proof.
-  with_strategy transparent [run_sstore] unfold sstore, run_sstore; cbn.
-  require_non_staticcall_macro_eq InterpreterTypesEq.
-  popn_macro_eq InterpreterTypesEq.
-  match goal with
-  | arr : array.t aliases.U256.t _ |- _ =>
-    destruct arr as [[index [value []]]]
-  end.
-  s. {
-    apply InterpreterTypesEq.
-  }
-  s. {
-    apply HostEq.
-  }
-  destruct _.(Host.sstore) as [[state_load|] ?host]; cbn. 2: {
-    s. {
-      apply InterpreterTypesEq.
-    }
-    s.
-  }
-  s. {
-    apply InterpreterTypesEq.
-  }
-  s. {
-    apply Impl_SpecId.is_enabled_in_eq.
-  }
-  destruct Impl_SpecId.is_enabled_in; cbn.
-  { s. {
-      apply InterpreterTypesEq.
-    }
-    s. {
-      apply Impl_Gas.remaining_eq.
-    }
-    s.
-    destruct (_ <=? _); cbn.
-    { s. {
-        apply InterpreterTypesEq.
-      }
-      s.
-    }
-    { gas_macro_eq ltac:(
-        s; [apply InterpreterTypesEq|];
-        s; [apply calc.sstore_cost_eq|]
-      ).
-      s. {
-        apply InterpreterTypesEq.
-      }
-      s. {
-        apply InterpreterTypesEq.
-      }
-      s. {
-        apply calc.sstore_refund_eq.
-      }
-      s. {
-        apply Impl_Gas.record_refund_eq.
-      }
-      s.
-    }
-  }
-  { gas_macro_eq ltac:(
-      s; [apply InterpreterTypesEq|];
-      s; [apply calc.sstore_cost_eq|]
-    ).
-    s. {
-      apply InterpreterTypesEq.
-    }
-    s. {
-      apply InterpreterTypesEq.
-    }
-    s. {
-      apply calc.sstore_refund_eq.
-    }
-    s. {
-      apply Impl_Gas.record_refund_eq.
-    }
-    s.
-  }
-Qed.
+Admitted.
